# 数列求和

##### 1. 已知等差数列$\{a_n\}$的前$n$项和为$S_n$,且满足$a_4 \cdot x^2 - S_3 \cdot x + 2 \lt 0$的解集为$\left( \frac{2}{7} , 1 \right)$

(1) 求数列$\{a_n\}$的通项公式；

由韦达定理可知：
    \[ \frac{S_3}{a_4}=1+\frac{2}{7} \\\\
     \frac{2}{a_4}=1 \cdot \frac{2}{7} \]
又因为
    \[ \{a_n\}是等差数列 \]
所以
    \[ a_n=2n-1 \]

(2) 若数列$\{c_n\}$满足$c_n =  a_{2n} + 2^{a_n}$,求数列$\{c_n\}$的前$n$项和$T_n$

因为
    \[ a_{2n}=4n-1 \\\\
       2^{a_n}=2^{2n-1}  \]
所以
    \[ c_n=4n-1+2^{2n-1} \\\\
       T_n = 2n^2+n-\frac{2(1-4^n)}{3}  \]
    

##### 2. 设$S_n$是数列$\{a_n\}$的前$n$项和，已知$a_1 = 3, a_{n+1} = 2S_n + 3 \left(n \in \mathbb{N} \right)$.

(1) 求数列$\{a_n\}$的通项公式
    \[ a_{n+1}-a_n=2a_n \\\\
       \frac{a_{n+1}}{a_n}=3 \]
所以
    \[ a_n=3^n \]

(2) 令$b_n=(2n-1)a_n$，求数列$\{b_n\}$的前$n$项和$T_n$.
    \[ T_n=3+9+...+(2n-1) \cdot 3^n \\\\
        3T_n=9+...+ (2n-1) \cdot 3^{n+1} \]
所以
    \[ T_n=\frac{(2n-1)3^{n+1}-3}{2} \]